Switch back to separate Stream subtype

codegen/smithy-dafny-codegen/src/main/java/software/amazon/polymorph/smithydafny/DafnyApiCodegen.java
@@ -312,8 +312,8 @@ public class DafnyApiCodegen {
     if (blobShape.hasTrait(StreamingTrait.class)) {
       // TODO: need to handle @length too,
       // something like `forall produced | a.CanProduce(produced) :: min <= |Enumerated(produced)| <= max
-      // (which should have a simpler helper predicate version, especially when allowing for reference types)
-      return generateTypeSynonym(blobShapeId, "Enumerator<bytes>");
+      // (which should have a simpler helper predicate version, especially when allowing for refeStandardLibrary.Actionsrence types)
+      return generateTypeSynonym(blobShapeId, "Stream<bytes>");
     } else {
       return generateSubsetType(blobShapeId, "seq<uint8>", lengthConstraint);
     }
