TestModels/dafny-dependencies/StandardLibrary/src/DynamicArray.dfy
@@ -80,7 +80,7 @@ module {:options "--function-syntax:4"} Std.DynamicArray {
     method Put(index: nat, element: A)
       requires index < size
       requires Valid?()
-      reads this, Repr
+      // reads this, Repr
       modifies Repr, `items
       ensures Valid?()
       ensures fresh(Repr - old(Repr))
@@ -99,7 +99,7 @@ module {:options "--function-syntax:4"} Std.DynamicArray {
     method Ensure(reserved: nat, defaultValue: A)
       requires Valid?()
       ensures Valid?()
-      reads this, Repr
+      // reads this, Repr
       modifies Repr
       ensures size == old(size)
       ensures items == old(items)
@@ -140,7 +140,7 @@ module {:options "--function-syntax:4"} Std.DynamicArray {
     method PushFast(element: A)
       requires Valid?()
       requires size < capacity
-      reads this, Repr
+      // reads this, Repr
       modifies Repr
       ensures Valid?()
       ensures fresh(Repr - old(Repr))
@@ -161,7 +161,7 @@ module {:options "--function-syntax:4"} Std.DynamicArray {
      */
     method Push(element: A)
       requires Valid?()
-      reads this, Repr
+      // reads this, Repr
       modifies Repr
       ensures Valid?()
       ensures fresh(Repr - old(Repr))
@@ -178,7 +178,7 @@ module {:options "--function-syntax:4"} Std.DynamicArray {
     method Realloc(defaultValue: A, newCapacity: nat)
       requires Valid?()
       requires newCapacity > capacity
-      reads this, Repr
+      // reads this, Repr
       modifies `capacity, `data, `Repr, data
       ensures Valid?()
       ensures capacity == newCapacity
@@ -197,7 +197,7 @@ module {:options "--function-syntax:4"} Std.DynamicArray {
 
     method ReallocDefault(defaultValue: A)
       requires Valid?()
-      reads this, Repr
+      // reads this, Repr
       modifies `capacity, `data, `Repr, data
       ensures Valid?()
       ensures fresh(data)
@@ -211,7 +211,7 @@ module {:options "--function-syntax:4"} Std.DynamicArray {
       requires count as int <= newData.Length
       requires count <= capacity
       requires data.Length == capacity as int
-      reads this, Repr, data, newData
+      // reads this, Repr, data, newData
       modifies data
       ensures data[..count] == newData[..count]
       ensures data[count..] == old(data[count..])
