TestModels/dafny-dependencies/StandardLibrary/src/GenericAction.dfy
@@ -26,7 +26,7 @@ module {:options "--function-syntax:4"} Std.GenericActions {
 
     method Invoke(t: T) returns (r: R) 
       requires Requires(t)
-      reads Reads(t)
+      // reads Reads(t)
       modifies Modifies(t)
       decreases Decreases(t).Ordinal()
       ensures Ensures(t, r)
